ex_1.5 e 1.6

Labs/Lab_5/Ex_1.dfy
@@ -1,13 +1,23 @@
+function filter(s: seq<int>):seq<int>
+{
+    if (s == [])
+        then []
+        else if s[0] < 0
+                then filter(s[1..])
+                else [s[0]] + filter(s[1..])
+}
+
+
 
 class Node {
 
     var val : int
     var next : Node?
 
-    ghost var footprint : set<Node>
-    ghost var list : seq<int> 
+    ghost var footprint : set<Node> //atributos
+    ghost var list : seq<int>       //usados para justificação
 
-    ghost function Valid() : bool 
+    ghost function Valid() : bool //apenas serve para justificação
         reads this, footprint 
         decreases footprint
     {
@@ -53,5 +63,94 @@ class Node {
       r.footprint := {r} + this.footprint;
     }
 
+    method append(i:int)
+    requires Valid()
+    ensures this.list == old(this.list) + [i]
+    && fresh(footprint - old(footprint))
 
+    decreases footprint
+    modifies footprint
+    {
+        if(this.next == null){
+            var r:= new Node(i);
+            this.next := r;
+            this.footprint := {this, r};
+            this.list := [this.val, i];
+        }else{
+            this.next.append(i);
+            this.footprint := {this} + this.next.footprint;
+            this.list := [this.val] + this.next.list;
+        }
+
+    }
+
+    
+    method find(i: int) returns (b: bool)
+    requires Valid()
+    ensures b == (i in this.list)
+    
+    {
+      var cur := this;
+      b := false;
+      ghost var listaux := [];
+      while(cur != null)
+      invariant cur != null ==> cur.Valid()
+      invariant !(i in listaux)
+      invariant cur != null ==> this.list == listaux + cur.list
+      invariant cur == null ==> this.list == listaux
+      
+      decreases if (cur != null) then cur.footprint else{}
+      {
+        if(cur.val == i){
+            b:=true;
+            return;
+        }
+        listaux := listaux + [cur.val];
+        cur:=cur.next;
+      }
+      
+    }
+
+    method filter() returns (r:Node?)
+    requires Valid()
+    ensures r!=null ==> r.Valid()
+    ensures r!=null ==> r.footprint <= old(this.footprint)
+    ensures r!=null ==> r.list == filter(old(this.list))
+    ensures r==null ==> filter(old(this.list)) == []
+    modifies footprint
+    decreases footprint
+    {
+        if (this.next == null) {
+            if (this.val < 0){
+                r:= null;
+                return;
+            }else{
+                r:= this;
+                return;
+            }
+        }else{
+            var aux := this.next.filter();
+            if (this.val < 0){
+                r:= aux;
+                return;
+            }else{
+                if (aux != null){
+                    r := this;
+                    r.next:=aux;
+                    r.list := [r.val] + aux.list;
+                    r.footprint := {r} + aux.footprint;
+                    return;
+                    }else{
+                        r := this;
+                        r.next:=null;
+                        r.list := [r.val];
+                        r.footprint := {r};
+                        return;
+                }
+            }
+            return;
+        }
+    }
 }
+
+
